Simu/Tra.v
@@ -18,10 +18,12 @@ Axiom first_unused_ident: unit -> ident.
 Definition self_id: ident := pos_of_str "self".
 Definition out_id: ident := pos_of_str "out".
 Definition main_id: ident := pos_of_str "main".
-Definition step_id (id: ident): ident :=
+Definition prefix (pref id: ident): ident :=
+  pos_of_str ((pos_to_str pref) ++ "_" ++ (pos_to_str id)).
+Definition step_id (id: ident): ident := 
   pos_of_str ("step_" ++ (pos_to_str id)).
-Definition reset_id (id: ident): ident :=
-  pos_of_str ("reset_" ++ (pos_to_str id)).
+(* Definition reset_id (id: ident): ident := *)
+(*   pos_of_str ("reset_" ++ (pos_to_str id)). *)
 
 (* TRANSLATION *)
 Definition type_of_inst (o: ident): typ :=
@@ -49,9 +51,9 @@ Definition translate_exp (c: class) (m: method) (e: exp): Clight.expr :=
   match e with
   | Var x ty =>
     if existsb (fun out => ident_eqb (fst out) x) m.(m_out) then
-      deref_field out_id (step_id c.(c_name)) x ty
+      deref_field out_id (prefix m.(m_name) c.(c_name)) x ty
     else
-      Clight.Evar x ty  
+      Clight.Etempvar x ty  
   | State x ty => deref_field self_id c.(c_name) x ty
   | Const c ty => translate_const c ty
   end.
@@ -69,25 +71,31 @@ Definition funcall (f: ident) (args: list Clight.expr) : Clight.statement :=
 
 Definition assign (x: ident) (ty: typ) (clsid: ident) (m: method): Clight.expr -> Clight.statement :=
   if existsb (fun out => ident_eqb (fst out) x) m.(m_out) then
-      Clight.Sassign (deref_field out_id (step_id clsid) x ty)
-    else
-      Clight.Sset x.
+    Clight.Sassign (deref_field out_id (prefix m.(m_name) clsid) x ty)
+  else
+    Clight.Sset x.
 
 (* Definition binded_funcall (bind temp f: ident) (ty: typ) (args: list Clight.expr) *)
 (*   : Clight.statement := *)
 (*    Clight.Ssequence (funcall (Some temp) f ty args) *)
 (*                     (assign bind ty (Clight.Etempvar temp ty)). *)
 
-Definition ptr_obj (owner: option ident) (cls obj: ident): Clight.expr :=
-  Clight.Eaddrof
-    ((match owner with
-      | Some owner => deref_field self_id owner
-      | None => Clight.Evar
-      end) obj (type_of_inst cls))
-    (type_of_inst_p cls).  
+Definition ptr_obj (owner: ident) (cls obj: ident): Clight.expr :=
+  Clight.Eaddrof (deref_field self_id owner obj (type_of_inst cls)) (type_of_inst_p cls).  
+
+Definition funcall_assign
+           (ys: list (ident * typ)) (owner: ident) (obj: ident) (tyout: typ) (m: method)
+           : Clight.statement :=
+  fold_right
+    (fun y s =>
+       let '((y, ty), (y', _)) := y in
+       let assign_out := assign y ty owner m (Clight.Efield (Clight.Evar obj tyout) y' ty) in
+       Clight.Ssequence assign_out s
+    ) Clight.Sskip (combine ys m.(m_out)).
 
 Definition binded_funcall
-           (prog: program) (ys: list (ident * typ)) (owner cls f obj: ident) (args: list Clight.expr)
+           (prog: program) (ys: list (ident * typ)) (owner: ident)
+           (cls f obj: ident) (args: list Clight.expr)
   : Clight.statement :=
   match find_class cls prog with
   | Some (c, _) =>
@@ -95,15 +103,10 @@ Definition binded_funcall
     | Some m =>
       let tyout := type_of_inst obj in
       let out := Clight.Eaddrof (Clight.Evar obj tyout) (pointer_of tyout) in 
-      let args := ptr_obj (Some owner) cls obj :: args ++ [out] in
+      let args := ptr_obj owner cls obj :: args ++ [out] in
       Clight.Ssequence
         (funcall f args)
-        (fold_right
-           (fun y s =>
-              let '((y, ty), (y', _)) := y in
-              let assign_out := assign y ty owner m (Clight.Efield (Clight.Evar obj tyout) y' ty) in
-              Clight.Ssequence assign_out s
-           ) Clight.Sskip (combine ys m.(m_out)))
+        (funcall_assign ys owner obj tyout m)
     | None => Clight.Sskip
     end
   | None => Clight.Sskip
@@ -112,32 +115,34 @@ Definition binded_funcall
 (* Definition reset_call (owner: option ident) (cls obj: ident): Clight.statement := *)
 (*   funcall (reset_id cls) [ptr_obj owner cls obj]. *)
 
-Definition make_in_arg (arg: ident * typ): Clight.expr :=
-  let (x, ty) := arg in
-  Clight.Evar x ty.
-(* Definition make_out_arg (arg: ident * typ): Clight.expr := *)
-(*   let (x, ty) := arg in *)
-(*   Clight.Eaddrof (Clight.Evar x ty) (pointer_of ty). *)
 
 (** 
 Statement conversion keeps track of the produced temporaries (function calls).
 [c] represents the current class.
  *)
-Fixpoint translate_stmt (prog: program) (c: class) (m: method) (s: stmt): Clight.statement :=
+Fixpoint translate_stmt
+         (out_structs: list (ident * ident * ident)) (prog: program) (c: class) (m: method) (s: stmt)
+  : list (ident * ident * ident) * Clight.statement :=
   match s with
   | Assign x e =>
-    assign x (typeof e) c.(c_name) m (translate_exp c m e) 
+    (out_structs,
+     assign x (typeof e) c.(c_name) m (translate_exp c m e)) 
   | AssignSt x e =>
-    Clight.Sassign (deref_field self_id c.(c_name) x (typeof e)) (translate_exp c m e)
+    (out_structs,
+     Clight.Sassign (deref_field self_id c.(c_name) x (typeof e)) (translate_exp c m e))
   | Ifte e s1 s2 =>
-    Clight.Sifthenelse (translate_exp c m e)
-                       (translate_stmt prog c m s1) (translate_stmt prog c m s2)
+    let (os1, s1) := translate_stmt out_structs prog c m s1 in
+    let (os2, s2) := translate_stmt os1 prog c m s2 in
+    (os2, Clight.Sifthenelse (translate_exp c m e) s1 s2) 
   | Comp s1 s2 =>
-    Clight.Ssequence (translate_stmt prog c m s1) (translate_stmt prog c m s2)
+    let (os1, s1) := translate_stmt out_structs prog c m s1 in
+    let (os2, s2) := translate_stmt os1 prog c m s2 in
+    (os2, Clight.Ssequence s1 s2)
   | Call ys cls f o es =>
-    binded_funcall prog ys c.(c_name) cls f o (map (translate_exp c m) es)  
+    ((o, cls, f) :: out_structs,
+     binded_funcall prog ys c.(c_name) cls f o (map (translate_exp c m) es))  
   | Skip =>
-    Clight.Sskip
+    (out_structs, Clight.Sskip)
   end.
 
 (* Definition return_some (s: Clight.statement) (out: ident * typ): Clight.statement := *)
@@ -156,43 +161,53 @@ Definition fundef
   let f := Clight.mkfunction ty AST.cc_default ins vars temps body in
   @AST.Gfun Clight.fundef typ (Ctypes.Internal f).
 
-Definition make_fun
+Definition make_fundef
            (self: ident * typ) (ins: list (ident * typ)) (out: ident * typ)
            (vars temps: list (ident * typ)) (body: Clight.statement)
   : AST.globdef Clight.fundef Ctypes.type :=
   let body := return_none body in
   fundef (self :: ins ++ [out]) vars temps Ctypes.Tvoid body.
 
+Definition make_out_vars (out_vars: list (ident * ident * ident)): list (ident * typ) :=
+  map (fun ocf =>
+         let '(o, cid, f) := ocf in
+         (o, type_of_inst (prefix f cid))
+      ) out_vars.
+
 Definition translate_method (prog: program) (c: class) (m: method)
   : ident * AST.globdef Clight.fundef Ctypes.type :=
-  let body := translate_stmt prog c m m.(m_body) in
+  let (out_vars, body) := translate_stmt [] prog c m m.(m_body) in
   let self := (self_id, type_of_inst_p c.(c_name)) in
-  let out := make_out_struct m.(m_out) in
-  make_fun self m.(m_in) out [] m.(m_vars) body.
+  let out := (out_id, type_of_inst_p (prefix m.(m_name) c.(c_name))) in
+  (prefix m.(m_name) c.(c_name),
+   make_fundef self m.(m_in) out (make_out_vars out_vars) m.(m_vars) body).
+
+Definition make_methods (prog: program) (c: class)
+  : list (ident * AST.globdef Clight.fundef Ctypes.type) :=
+  map (translate_method prog c) c.(c_methods).
 
 Definition translate_obj (obj: ident * ident): (ident * typ) :=
   let (o, c) := obj in
   (o, type_of_inst c).
 
-Definition make_struct (cls: ident) (members: list (ident * typ))
-  : Ctypes.composite_definition :=
-  Ctypes.Composite cls Ctypes.Struct members Ctypes.noattr.
-
 Definition make_members (c: class): Ctypes.members :=
   c.(c_mems) ++ map translate_obj c.(c_objs).
 
-Definition translate_class (c: class)
-  : Ctypes.composite_definition * (ident * AST.globdef Clight.fundef Ctypes.type) :=
-  let members := make_members c in
-  match c with
-    mk_class c_name c_input c_output c_vars c_mems c_objs c_step =>
-    let members := c_mems ++ objs in
-    let step := translate_stmt c_name c_step in
-    let self := (self_id, type_of_inst_p c_name) in
-    let cl_struct := make_struct c_name members in
-    let cl_step := (step_id c_name, make_step self (nelist2list c_input) (nelist2list c_output) c_vars step) in
-    (cl_struct, cl_step)
-  end.
+Definition make_struct (c: class): Ctypes.composite_definition :=
+  Ctypes.Composite c.(c_name) Ctypes.Struct (make_members c) Ctypes.noattr.
+
+Definition translate_out (c: class) (m: method): Ctypes.composite_definition :=
+  Ctypes.Composite (prefix m.(m_name) c.(c_name)) Ctypes.Struct m.(m_out) Ctypes.noattr.
+
+Definition make_out (c: class): list Ctypes.composite_definition :=
+  map (translate_out c) c.(c_methods).
+
+Definition translate_class (prog: program) (c: class)
+  : list Ctypes.composite_definition * list (ident * AST.globdef Clight.fundef Ctypes.type) :=
+  let methods := make_methods prog c in
+  let class_struct := make_struct c in
+  let out_structs := make_out c in   
+  (class_struct :: out_structs, methods).
 
 Definition glob_id (id: ident): ident :=
   pos_of_str ("_" ++ (pos_to_str id)).
@@ -200,14 +215,35 @@ Definition glob_bind (bind: ident * typ): ident * typ :=
   let (x, ty) := bind in
   (glob_id x, ty).
 
-Definition make_main (node: ident) (f: ident) (ins: list (ident * typ)) (outs: list (ident * typ))
+Definition make_in_arg (arg: ident * typ): Clight.expr :=
+  let (x, ty) := arg in
+  Clight.Evar x ty.
+(* Definition make_out_arg (arg: ident * typ): Clight.expr := *)
+(*   let (x, ty) := arg in *)
+(*   Clight.Eaddrof (Clight.Evar x ty) (pointer_of ty). *)
+
+Definition make_main
+           (prog: program) (node: ident) (ins: list (ident * typ))
+           (outs: list (ident * typ)) (m: method)
   : AST.globdef Clight.fundef Ctypes.type :=
+  let out_struct := step_id node in
   let args_in := List.map make_in_arg ins in
-  let args_out := List.map make_out_arg outs in
-  let step := step_call None node f (args_in ++ args_out) in
+  let tyout := type_of_inst (step_id node) in
+  let out := Clight.Eaddrof (Clight.Evar out_struct tyout) (pointer_of tyout) in 
+  let args := (Clight.Eaddrof (Clight.Evar (glob_id node) (type_of_inst node)) (type_of_inst_p node))
+                :: args_in ++ [out] in
+  let step := Clight.Ssequence
+                (funcall (step_id node) args)
+                (fold_right
+                   (fun y s =>
+                      let '((y, ty), (y', _)) := y in
+                      let assign_out := Clight.Sassign (Clight.Evar y ty)
+                                                       (Clight.Efield (Clight.Evar out_struct tyout) y' ty) in
+                      Clight.Ssequence assign_out s
+    ) Clight.Sskip (combine outs m.(m_out))) in
   let loop := Clight.Sloop ((* Clight.Ssequence wait *) step) Clight.Sskip in
   let body := return_zero ((* Clight.Ssequence (reset_call None node f) *) loop) in
-  fundef [] [] Ctypes.type_int32s body.
+  fundef [] [(out_struct, type_of_inst (step_id node))] [] Ctypes.type_int32s body.
 
 Definition vardef (init volatile: bool) (x: ident * typ): ident * AST.globdef Clight.fundef Ctypes.type :=
   let (x, ty) := x in
@@ -215,19 +251,24 @@ Definition vardef (init volatile: bool) (x: ident * typ): ident * AST.globdef Cl
   (x, @AST.Gvar Clight.fundef _
                 (AST.mkglobvar ty' (if init then [AST.Init_space Z0] else []) false volatile)).
 
-Definition translate (p: program) (main_node: ident): Errors.res Clight.program :=
-  match find_class main_node p with
-  | Some (cls, _) =>
-    let f := glob_id main_node in
-    let ins := map glob_bind (nelist2list cls.(c_input)) in
-    let outs := map glob_bind (nelist2list cls.(c_output)) in
-    let main := make_main main_node f ins outs in
-    let cs := List.map translate_class p in
-    let f_gvar := vardef true false (f, type_of_inst main_node) in
-    let o_gvars := map (vardef true true) outs in
-    let i_gvars := map (vardef true true) ins in
-    let (structs, steps) := split cs in
-    let gdefs := f_gvar :: o_gvars ++ i_gvars ++ steps ++ [(main_id, main)] in
-    Ctypes.make_program structs gdefs [] main_id                    
+Print List.
+Definition translate (prog: program) (main_node: ident): Errors.res Clight.program :=
+  match find_class main_node prog with
+  | Some (c, _) =>
+    match find_method (step_id main_node) c.(c_methods) with
+    | Some m =>
+      let f := glob_id main_node in
+      let ins := map glob_bind m.(m_in) in
+      let outs := map glob_bind m.(m_out) in
+      let main := make_main prog main_node ins outs m in
+      let cs := List.map (translate_class prog) prog.(p_classes) in
+      let f_gvar := vardef true false (f, type_of_inst main_node) in
+      let o_gvars := map (vardef true true) outs in
+      let i_gvars := map (vardef true true) ins in
+      let (structs, funs) := split cs in
+      let gdefs := f_gvar :: o_gvars ++ i_gvars ++ (concat funs) ++ [(main_id, main)] in
+      Ctypes.make_program (concat structs) gdefs [] main_id
+    | None => Errors.Error (Errors.msg "unfound step function")
+    end
   | None => Errors.Error (Errors.msg "undefined node")
   end.
